PREFIX : <https://linked.data.gov.au/def/addrcm-rec/>
PREFIX cs: <https://linked.data.gov.au/def/addrcm-rec>
PREFIX owl: <http://www.w3.org/2002/07/owl#>
PREFIX rdfs: <http://www.w3.org/2000/01/rdf-schema#>
PREFIX reg: <http://purl.org/linked-data/registry#>
PREFIX schema: <https://schema.org/>
PREFIX skos: <http://www.w3.org/2004/02/skos/core#>
PREFIX status: <https://linked.data.gov.au/def/reg-statuses/>
PREFIX themes: <https://linked.data.gov.au/def/fsdf/themes/>
PREFIX xsd: <http://www.w3.org/2001/XMLSchema#>

:generalGoodPractice
    a skos:Collection ;
    rdfs:isDefinedBy cs: ;
    skos:definition ""@en ;
    skos:inScheme cs: ;
    skos:member
        :objectivesForPublicGood ,
        :iso19160-1-profile ,
        :intellectualPropertyRights ,
        :facilitateAssignment ,
        :keepingAddressDataInSynch ;
    skos:prefLabel "General Good Practice"@en ;
.

:principles
    a skos:Collection ;
    rdfs:isDefinedBy cs: ;
    skos:definition ""@en ;
    skos:inScheme cs: ;
    skos:member
        :unambiguity ,
        :equivalentDigitalRecord ,
        :updateAddressData ,
        :conformsToIso19160-1 ,
        :conformsToIso19160-4 ,
        :conformsToIso19160-3 ,
        :sharing ;
    skos:prefLabel "Principles"@en ;
.

:generalGovernanceFramework
    a skos:Collection ;
    rdfs:isDefinedBy cs: ;
    skos:definition ""@en ;
    skos:inScheme cs: ;
    skos:member
        :policiesSupportObjectivesAndContext ;
    skos:prefLabel "General Governance Framework"@en ;
.

:processes
    a skos:Collection ;
    rdfs:isDefinedBy cs: ;
    skos:definition ""@en ;
    skos:inScheme cs: ;
    skos:member
        :consultationProcess ;
    skos:prefLabel "Processes"@en ;
.

:conformsToIso19160-1
    a skos:Concept ;
    skos:notation "9"^^xsd:integer ;
    skos:definition "Address data should conform to ISO 19160-1:2015, or a profile thereof"@en ;
    skos:inScheme cs: ;
    skos:prefLabel "Conforms To ISO 19160-1"@en ;
    skos:topConceptOf cs: ;
.

:conformsToIso19160-3
    a skos:Concept ;
    skos:notation "11"^^xsd:integer ;
    skos:definition "The quality of address data should be described conformant to ISO 19160-3:2020, or a profile thereof"@en ;
    skos:inScheme cs: ;
    skos:prefLabel "Conforms To ISO 19160-3"@en ;
    skos:topConceptOf cs: ;
.

:conformsToIso19160-4
    a skos:Concept ;
    skos:notation "10"^^xsd:integer ;
    skos:definition "For postal addressing, address data should conform to ISO 19160-4:2017, or a profile thereof"@en ;
    skos:inScheme cs: ;
    skos:prefLabel "Conforms To ISO 19160-4"@en ;
    skos:topConceptOf cs: ;
.

:consultationProcess
    a skos:Concept ;
    skos:notation "14"^^xsd:integer ;
    skos:definition "A governance framework should specify and coordinate a process for consultation when new address component values are assigned or changed due to maintenance"@en ;
    skos:inScheme cs: ;
    skos:prefLabel "Consultation Process"@en ;
    skos:topConceptOf cs: ;
.

:equivalentDigitalRecord
    a skos:Concept ;
    skos:notation "7"^^xsd:integer ;
    skos:definition "TODO: add definition"@en ;
    skos:inScheme cs: ;
    skos:prefLabel "Equivalent Digital Record"@en ;
    skos:topConceptOf cs: ;
.

:facilitateAssignment
    a skos:Concept ;
    skos:notation "4"^^xsd:integer ;
    skos:definition "A good practice should specify a method for assigning values to address components that could be automated to speed up or facilitate address assignment and maintenance"@en ;
    skos:example "EXAMPLE 19 AS/NZS 4819:2011, Rural and urban addressing, contains a clause for addressing rural properties based on the measured distance along the road, from a defined datum point, the accessway of the property is, with odd numbers on the left side of the road and even numbers on the right." ;
    skos:inScheme cs: ;
    skos:prefLabel "Facilitate Assignment"@en ;
    skos:topConceptOf cs: ;
.

:intellectualPropertyRights
    a skos:Concept ;
    skos:notation "3"^^xsd:integer ;
    skos:definition "A good practice should specify to whom the intellectual property rights of the address assignment method and the address data belong. At the least, government organizations should have free access to the address data for services to ensure the health, safety and welfare of the public."@en ;
    skos:inScheme cs: ;
    skos:prefLabel "Intellectual Property Rights"@en ;
    skos:topConceptOf cs: ;
.

:iso19160-1-profile
    a skos:Concept ;
    skos:notation "2"^^xsd:integer ;
    skos:definition "The conceptual model that describes classes (types) of addresses assigned and maintained through the good practice should conform to ISO 19160-1:2015"@en ;
    skos:example "The draft NZ profile of ISO 19160-1:2015 describes its conformance to ISO 19160-1:2015. The NZ profile defines six address classes: Thoroughfare, Water, Service Delivery, Rural Post Delivery, Thoroughfare4819, and Water4819. New addresses (excluding NZ Post addresses for service delivery and rural post delivery) quality assured by the LINZ address team are assessed against the Thoroughfare4819 and Water4819 classes, and these classes align with the requirements in AS/NZS 4819:2011" ;
    skos:inScheme cs: ;
    skos:prefLabel "ISO 19160-1 Profile"@en ;
    skos:scopeNote """NOTE 1 Amongst others, ISO 19160-1:2015 requires that a conformant address model clearly specifies how the position of an address is represented in the model. ISO 19160-1:2015 provides two ways for doing this: 1) an address has coordinates to specify its position; 2) the position of the address is inferred from the addressed object. [SOURCE: ISO 19160-1:2015, 6.1]

NOTE 2 Postal addresses are defined and described in ISO 19160-4:2017, a profile of ISO 19160-1:2015.""" ;
    skos:topConceptOf cs: ;
.

:keepingAddressDataInSynch
    a skos:Concept ;
    skos:notation "5"^^xsd:integer ;
    skos:definition "A good practice should specify a method for keeping addresses in the physical world in synch with address data."@en ;
    skos:inScheme cs: ;
    skos:prefLabel "Keeping Address Data In Synch"@en ;
    skos:topConceptOf cs: ;
.

:objectivesForPublicGood
    a skos:Concept ;
    skos:notation "1"^^xsd:integer ;
    skos:definition "An objective should specify that the assignment and maintenance of addresses is done with the purpose of benefitting governance and society and thereby achieving public good"@en ;
    skos:inScheme cs: ;
    skos:prefLabel "Objectives For Public Good"@en ;
    skos:scopeNote "Making address assignment and maintenance data open benefits governance and society by enhancing transparency, facilitating efficient urban planning, infrastructure development, emergency response, and ensuring equitable access to essential services, ultimately contributing to the public good" ;
    skos:topConceptOf cs: ;
.

:policiesSupportObjectivesAndContext
    a skos:Concept ;
    skos:notation "13"^^xsd:integer ;
    skos:definition "The policies should support the objectives and context"@en ;
    skos:inScheme cs: ;
    skos:prefLabel "Policies Support Objectives And Context"@en ;
    skos:topConceptOf cs: ;
.

:sharing
    a skos:Concept ;
    skos:notation "12"^^xsd:integer ;
    skos:definition "In the case of digital address data, the data should be shared through address retrieval solutions that preserve and maintain data integrity, e.g., through spreadsheets or APIs"@en ;
    skos:inScheme cs: ;
    skos:prefLabel "Sharing"@en ;
    skos:topConceptOf cs: ;
.

:unambiguity
    a skos:Concept ;
    skos:notation "6"^^xsd:integer ;
    skos:definition """An address shall be assigned to an addressable object in the physical world so that it allows the unambiguous determination of the object for purposes of identification and location (ISO 19160-1:2015).

A thoroughfare address shall be assigned that conforms to the list of mandatory components to enable unambiguity, and enable it to be readily located."""@en ;
    skos:inScheme cs: ;
    skos:prefLabel "Unambiguity"@en ;
    skos:scopeNote "NOTE 1 The position of an address can be represented in two ways: 1) The position is specified by coordinates in the ‘position’ attribute. 2) The position is inferred from the addressed object. See 6.1 in ISO 19160-1:2015." ;
    skos:topConceptOf cs: ;
.

:updateAddressData
    a skos:Concept ;
    skos:notation "8"^^xsd:integer ;
    skos:definition "TODO: add definition"@en ;
    skos:inScheme cs: ;
    skos:prefLabel "Update Address Data"@en ;
    skos:topConceptOf cs: ;
.

<https://linked.data.gov.au/org/qsi>
    a schema:Organization ;
    schema:name "Queensland Spatial Information" ;
    schema:url "https://www.resources.qld.gov.au/data-mapping"^^xsd:anyURI ;
.

<https://linked.data.gov.au/org/icsm>
    a schema:Organization ;
    schema:name "Intergovernmental Committee on Surveying & Mapping" ;
    schema:url "https://icsm.gov.au"^^xsd:anyURI ;
.

cs:
    a skos:ConceptScheme ;
    reg:status status:experimental ;
    owl:versionIRI :1.0 ;
    owl:versionInfo "1.0" ;
    skos:definition "Requirements and Recommendations for Address Creation & Maintenance"@en ;
    skos:hasTopConcept
        :conformsToIso19160-1 ,
        :conformsToIso19160-3 ,
        :conformsToIso19160-4 ,
        :consultationProcess ,
        :equivalentDigitalRecord ,
        :facilitateAssignment ,
        :intellectualPropertyRights ,
        :iso19160-1-profile ,
        :keepingAddressDataInSynch ,
        :objectivesForPublicGood ,
        :policiesSupportObjectivesAndContext ,
        :sharing ,
        :unambiguity ,
        :updateAddressData ;
    skos:historyNote "This vocabulary was created as part of the authoring of the Intergovernmental Committee on Surveying & Mapping's Australian Addressing Creation & Maintenance Standard in 2024" ;
    skos:prefLabel "Address Creation & Maintenance Recommendations"@en ;
    skos:scopeNote "The Recommendations contained in this vocabulary are referred to within the Intergovernmental Committee on Surveying & Mapping's Australian Addressing Creation & Maintenance Standard" ;
    schema:contributor <https://linked.data.gov.au/org/qsi> ;
    schema:copyrightNotice "(c) Intergovernmental Committee on Surveying & Mapping, 2024" ;
    schema:creator <https://linked.data.gov.au/org/icsm> ;
    schema:dateCreated "2024-10-09"^^xsd:date ;
    schema:dateModified "2024-10-09"^^xsd:date ;
    schema:keywords themes:geocoded-addressing ;
    schema:license <https://rdflicense.linkeddata.es/rdflicense/cc-by4.0> ;
    schema:publisher <https://linked.data.gov.au/org/icsm> ;
.
